extraction/theories/MidlangPretty.v
@@ -1,24 +1,24 @@
 From ConCert.Execution Require Import Blockchain.
 From ConCert.Execution Require Import Serializable.
 From ConCert.Execution Require Import Containers.
-From ConCert.Execution Require Import Congress.
 From ConCert.Extraction Require Import Certified.
-From ConCert Require Import MyEnv.
 
+From Coq Require Import Ascii.
 From Coq Require Import List.
 From Coq Require Import String.
-From Coq Require Import ZArith.
 
-From MetaCoq.SafeChecker Require Import Loader PCUICSafeChecker SafeTemplateChecker.
+From MetaCoq.SafeChecker Require Import PCUICSafeChecker.
 From MetaCoq.Template Require Import All.
 From MetaCoq.Erasure Require Import Debox Loader SafeTemplateErasure EAst EAstUtils ETyping.
 
 Import ListNotations.
 Import MonadNotation.
 
+Local Open Scope string.
+
 Record PrettyPrinterState :=
   {
-    indent : nat;
+    indent_stack : list nat;
     output : string
   }.
 
@@ -32,100 +32,318 @@ Instance Monad_PrettyPrinter : Monad PrettyPrinter :=
        | inr (a, pps) => f a pps
        end |}.
 
-Definition printer_fail (str : string) : PrettyPrinter unit :=
-  fun pps => inl str.
-
-(*
-Inductive PrettyPrinter A :=
-| pp_error (msg : string)
-| pp_print (f : PrettyPrinterState -> string + A * PrettyPrinterState).
-
-Arguments pp_print {_}.
-Arguments pp_error {_}.
-
-Instance Monad_PrettyPrinter : Monad PrettyPrinter :=
-  {| ret _ a := pp_print (fun pps => inr (a, pps));
-     bind _ _ m f :=
-       match m with
-       | pp_error msg => pp_error msg
-       | pp_print h =>
-         pp_print
-           (fun pps =>
-              match h pps with
-              | inl msg => inl msg
-              | inr (a, pps) =>
-                match f a with
-                | pp_error msg => inl msg
-                | pp_print g => g pps
-                end
-              end)
-       end |}.
-*)
-
-(*
-Definition State T A := T -> A * T.
-
-Instance Monad_State {T} : Monad (State T) :=
-  {| ret _ x t := (x, t);
-     bind _ _ a f x := let (t, x) := a x in f t x |}.
-
-Definition get_state {T} : State T T :=
-  fun t => (t, t).
-
-Definition set_state {T} (t : T) : State T unit :=
-  fun _ => (tt, t).
-
-Definition update_state {T} (f : T -> T) : State T unit :=
-  fun t => (tt, f t).
-
-Definition PrettyPrinter := State PrettyPrinterState.
-*)
+Definition printer_fail {A} (str : string) : PrettyPrinter A :=
+  fun pps => inl (str ++ nl ++ "failed after printing" ++ nl ++ (output pps)).
 
 Definition finish_print {A} (pp : PrettyPrinter A) : string + A * string :=
-  match pp {| indent := 0; output := "" |} with
+  match pp {| indent_stack := []; output := "" |} with
   | inl err => inl err
   | inr (a, pps) => inr (a, output pps)
   end.
 
-Definition update_indent (f : nat -> nat) : PrettyPrinter unit :=
-  fun pps => inr (tt, {| indent := f (indent pps); output := output pps |}).
+Definition get_indent : PrettyPrinter nat :=
+  fun pps => inr (hd 0 (indent_stack pps), pps).
 
-Definition inc_indent : PrettyPrinter unit :=
-  update_indent S.
+Definition update_indent (f : list nat -> list nat) : PrettyPrinter unit :=
+  fun pps => inr (tt, {| indent_stack := f (indent_stack pps); output := output pps |}).
 
-Definition dec_indent : PrettyPrinter unit :=
-  update_indent pred.
+Definition push_indent (n : nat) : PrettyPrinter unit :=
+  update_indent (cons n).
 
-Local Open Scope string.
+Definition pop_indent : PrettyPrinter unit :=
+  update_indent tl.
+
+Definition is_newline (c : ascii) : bool :=
+  match c with
+  | "010"%char => true
+  | _ => false
+  end.
+
+Definition last_line_length (s : string) : nat :=
+  (fix f (s : string) (result : nat) :=
+     match s with
+     | EmptyString => result
+     | String c s =>
+       if is_newline c then
+         f s 0
+       else
+         f s (S result)
+     end) s 0.
+
+Definition get_current_line_length : PrettyPrinter nat :=
+  fun pps => inr (last_line_length (output pps), pps).
+
 Definition update_output (f : string -> string) : PrettyPrinter unit :=
-  fun pps => inr (tt, {| indent := indent pps; output := f (output pps) |}).
+  fun pps => inr (tt, {| indent_stack := indent_stack pps; output := f (output pps) |}).
 
 Definition append (s : string) : PrettyPrinter unit :=
   update_output (fun o => o ++ s).
 
-Definition append_indent : PrettyPrinter unit :=
-  fun pps => inr (tt,
-                  {| indent := indent pps;
-                     output := output pps ++ concat "" (repeat "  " (indent pps)) |}).
+Definition append_nl : PrettyPrinter unit := append nl.
 
-Definition append_line (s : string) : PrettyPrinter unit :=
-  update_output (fun o => o ++ s ++ nl).
+Definition append_indent : PrettyPrinter unit :=
+  indent <- get_indent;;
+  append (concat "" (repeat " " indent)).
+
+Definition append_nl_and_indent : PrettyPrinter unit :=
+  append_nl;; append_indent.
+
+Definition replace_char (orig : Ascii.ascii) (new : Ascii.ascii) : string -> string :=
+  fix f s :=
+    match s with
+    | EmptyString => EmptyString
+    | String c s => if (c =? orig)%char then
+                      String new (f s)
+                    else
+                      String c (f s)
+    end.
+
+Definition printable_kername : kername -> string :=
+  replace_char "." "_".
 
 Local Open Scope list.
-Fixpoint print_term (Γ : context) (t : term) : PrettyPrinter unit :=
+
+Section PrintMidlang.
+
+Context (Σ : global_context).
+Context (indent_size := 2).
+
+Definition lookup_ind_decl ind i : PrettyPrinter one_inductive_body :=
+  match lookup_env Σ ind with
+  | Some (InductiveDecl {| ind_bodies := l |}) =>
+    match nth_error l i with
+    | Some body => ret body
+    | None => printer_fail ("could not find inductive " ++ string_of_nat i ++ " in inductive " ++ ind)
+    end
+  | _ => printer_fail ("could not find " ++ ind ++ " in environment")
+  end.
+
+Definition print_name (n : name) : PrettyPrinter unit :=
+  match n with
+  | nAnon => append "_"
+  | nNamed n => append n
+  end.
+
+Definition print_constructor_name (ind : inductive) (i : nat) : PrettyPrinter unit :=
+  oib <- lookup_ind_decl (inductive_mind ind) (inductive_ind ind);;
+  match nth_error (ind_ctors oib) i with
+  | Some (name, _, _) =>
+    append name
+    (*append (replace_char "." "_" (inductive_mind ind) ++ "_" ++ name)*)
+  | None =>
+    printer_fail (inductive_mind ind ++ " does not have a ctor " ++ string_of_nat i)
+  end.
+
+Definition print_parenthesized
+           (parenthesize : bool)
+           (print : PrettyPrinter unit) : PrettyPrinter unit :=
+  if parenthesize then
+    append "(";; print;; append ")"
+  else
+    print.
+
+Definition parenthesize_app_head (t : term) : bool :=
+  match t with
+  | tLambda _ _
+  | tLetIn _ _ _
+  | tCase _ _ _
+  | tFix _ _ => true
+  | _ => false
+  end.
+
+Definition parenthesize_app_arg (t : term) : bool :=
+  match t with
+  | tLambda _ _
+  | tLetIn _ _ _
+  | tApp _ _
+  | tCase _ _ _
+  | tProj _ _
+  | tFix _ _ => true
+  | _ => false
+  end.
+
+Definition parenthesize_case_discriminee (t : term) : bool :=
+  match t with
+  | tLetIn _ _ _
+  | tCase _ _ _ => true
+  | _ => false
+  end.
+
+Definition parenthesize_case_branch (t : term) : bool :=
+  false.
+
+Definition add_name (name : name) (Γ : list ident) : list ident :=
+  let name :=
+      match name with
+      | nAnon => "anon" (* fix *)
+      | nNamed name => name
+      end in
+  name :: Γ.
+
+Fixpoint print_term (Γ : list ident) (t : term) {struct t} : PrettyPrinter unit :=
   match t with
   | tBox _ => printer_fail "tBox"
-  | tRel _ => printer_fail "tRel"
+  | tRel n =>
+    match nth_error Γ n with
+    | Some name => append name
+    | None => printer_fail ("unbound tRel " ++ string_of_nat n)
+    end
   | tVar ident => printer_fail ("tVar " ++ ident)
-  | tEvar _ => printer_fail "unexpected evar"
-  | tLambda
+  | tEvar _ _ => printer_fail "unexpected evar"
+  | tLambda name t =>
+    append "\";;
+    print_name name;;
+    append " -> ";;
+    print_term (add_name name Γ) t
 
+  | tLetIn name value body =>
 
-Definition erase_check_debox_all_print
-           (TT : env string)
-           (decl_name : string)
-           (tys : list Ast.term)
-           (p : Ast.program) : string :=
-  let p := fix_program_universes p in
-  let deboxed := erase_check_debox_all TT p in
-  deboxed.
+    let_col <- get_current_line_length;;
+    append "let";;
+
+    push_indent (let_col + indent_size);;
+
+    let print_and_add_one Γ name value :=
+        append_nl_and_indent;;
+
+        print_name name;;
+        append " =";;
+
+        indent <- get_indent;;
+        push_indent (indent + indent_size);;
+        append_nl_and_indent;;
+
+        print_term Γ value;;
+
+        pop_indent;;
+
+        ret (add_name name Γ) in
+
+    Γ <- print_and_add_one Γ name value;;
+
+    (* Print in Midlang/Elm style, which collapses multiple lets into one *)
+    (fix print_lets Γ (t : term) :=
+       match t with
+       | tLetIn name value t =>
+         Γ <- print_and_add_one Γ name value;;
+         print_lets Γ t
+       | _ =>
+         pop_indent;; (* indent in let block *)
+
+         append_nl_and_indent;; (* indent to 'let' keyword *)
+         append "in";;
+
+         append_nl_and_indent;; (* body is indented to 'let'/'in' keyword as well *)
+         print_term Γ t;;
+         pop_indent
+       end) Γ body
+
+  | tApp head arg =>
+    print_parenthesized (parenthesize_app_head head) (print_term Γ head);;
+    append " ";;
+    print_parenthesized (parenthesize_app_arg arg) (print_term Γ arg)
+
+  | tConst name => append (printable_kername name)
+  | tConstruct ind i => print_constructor_name ind i
+
+  | tCase (ind, _) discriminee branches =>
+    case_col <- get_current_line_length;;
+    append "case ";;
+    print_parenthesized (parenthesize_case_discriminee discriminee)
+                        (print_term Γ discriminee);;
+    append " of";;
+
+    push_indent (case_col + indent_size);;
+
+    oib <- lookup_ind_decl (inductive_mind ind) (inductive_ind ind);;
+
+    (* Take care that this is structurally recursive... *)
+    (fix print_branches (branches : list (nat * term)) (ctor_names : list ident) :=
+       match branches, ctor_names with
+       | [], [] => ret tt
+       | (arity, t) :: branches, ctor_name :: ctor_names =>
+         append_nl_and_indent;;
+
+         ctor_indent <- get_indent;;
+         push_indent (ctor_indent + indent_size);;
+
+         append ctor_name;;
+
+         (fix print_branch (n : nat) (Γ : list ident) (t : term) {struct t} :=
+            match n with
+            | 0 =>
+              append " ->";;
+              append_nl_and_indent;;
+              print_parenthesized (parenthesize_case_branch t) (print_term Γ t)
+
+            | S n =>
+              match t with
+              | tLambda name t =>
+                append " ";;
+                print_name name;;
+                print_branch n (add_name name Γ) t
+
+              | _ => printer_fail "could not decompose branch"
+              end
+            end) arity Γ t;;
+
+         pop_indent;;
+
+         print_branches branches ctor_names
+       | _, _ => printer_fail "wrong number of case branches compared to inductive"
+       end) branches (map (fun '(name, _, _) => name) (ind_ctors oib));;
+
+    pop_indent
+
+  | tProj _ _ => printer_fail "tProj"
+  | tFix _ _ => printer_fail "tFix"
+  | tCoFix _ _ => printer_fail "Cannot handle cofix"
+  end.
+
+(*
+Fixpoint print_global_declarations (l : list (kername * global_decl)) : PrettyPrinter unit :=
+  match l with
+  | (name, decl) :: l =>
+    match decl with
+    | ConstantDecl
+*)
+
+End PrintMidlang.
+
+Local Open Scope nat.
+
+Inductive Msg :=
+| increment
+| decrement.
+
+(*
+Quote Recursively Definition test :=
+  (fun (state : nat) (maybe_msg : option Msg) =>
+    match maybe_msg with
+    | Some increment => Some (state + 1)
+    | Some decrement => Some (state - 1)
+    | _ => None
+    end).
+*)
+
+Quote Recursively Definition test :=
+  (let x := 5 in
+  let foo n := S n in
+  let y := 7 in
+  x + foo 3 + y + foo (foo x)).
+
+Compute erase_check_debox_all_print [] "foo" [] test.
+
+Definition test2 : string :=
+  match erase_check_debox_all [] test with
+  | CorrectDecl (Σ, (args, term)) =>
+    match finish_print (append_nl;; print_term Σ ["f"] term) with
+    | inl err => "Printer error: " ++ err
+    | inr (_, output) => output
+    end
+  | EnvError Σ (AlreadyDeclared id) => "Already declared: " ++ id
+  | EnvError Σ (IllFormedDecl id e) =>
+    "Type error: " ++ PCUICSafeChecker.string_of_type_error Σ e ++ ", while checking " ++ id
+  end.
+
+Compute test2.
