extraction/examples/CounterCertifiedExtraction.v
@@ -99,7 +99,7 @@ Definition TT : env string :=
 
 Quote Recursively Definition counter_syn := (unfolded counter).
 
-Time Eval vm_compute in (check_applied counter_syn).
+Time Eval vm_compute in (erase_and_check_applied counter_syn).
 Time Eval vm_compute in (erase_print_deboxed_all_applied TT counter_syn).
 
 (** We run the extraction procedure inside the [TemplateMonad]. It uses the certified erasure from [MetaCoq] and (so far uncertified) de-boxing procedure that removes application of boxes to constants and constructors. Even though the de-boxing is not certified yet, before removing boxes we check if constant is applied to all logical argument (i.e. proofs or types) and constructors are fully applied. In this case, it is safe to remove these applications. *)
