extraction/theories/MidlangExtract.v
@@ -1,0 +1,812 @@
+From ConCert.Execution Require Import Blockchain.
+From ConCert.Execution Require Import Serializable.
+From ConCert.Execution Require Import Containers.
+From ConCert.Extraction Require Import Certified.
+
+From Coq Require Import Arith.
+From Coq Require Import Ascii.
+From Coq Require Import List.
+From Coq Require Import String.
+
+From MetaCoq.SafeChecker Require Import PCUICSafeChecker SafeTemplateChecker.
+From MetaCoq.Template Require Import All.
+From MetaCoq.Erasure Require Import Debox Loader SafeTemplateErasure EAst EAstUtils ETyping.
+
+Module P := MetaCoq.PCUIC.PCUICAst.
+Module PT := MetaCoq.PCUIC.PCUICTyping.
+Module T2P := MetaCoq.PCUIC.TemplateToPCUIC.
+Module E := MetaCoq.Erasure.EAst.
+Module T := MetaCoq.Template.Ast.
+Module EF := MetaCoq.Erasure.SafeErasureFunction.
+
+Import ListNotations.
+Import MonadNotation.
+
+Local Open Scope string.
+
+Module Ex.
+  Record constant_body :=
+    { cst_type : P.term;
+      cst_body : option E.term; }.
+
+  Inductive global_decl :=
+  | ConstantDecl : constant_body -> global_decl
+  | InductiveDecl : P.mutual_inductive_body -> global_decl.
+
+  Definition global_env := list (kername * global_decl).
+
+  Fixpoint lookup_env (Σ : global_env) (id : ident) : option global_decl :=
+    match Σ with
+    | [] => None
+    | (name, decl) :: Σ => if ident_eq id name then Some decl else lookup_env Σ id
+    end.
+End Ex.
+
+Record PrettyPrinterState :=
+  {
+    indent_stack : list nat;
+    used_names : list ident;
+    output : string
+  }.
+
+Definition PrettyPrinter A := PrettyPrinterState -> (string + A * PrettyPrinterState).
+
+Instance Monad_PrettyPrinter : Monad PrettyPrinter :=
+  {| ret _ a pps := inr (a, pps);
+     bind _ _ m f pps :=
+       match m pps with
+       | inl err => inl err
+       | inr (a, pps) => f a pps
+       end |}.
+
+Definition printer_fail {A} (str : string) : PrettyPrinter A :=
+  fun pps => inl (str ++ nl ++ "failed after printing" ++ nl ++ (output pps)).
+
+Definition finish_print {A} (pp : PrettyPrinter A) : string + A * string :=
+  match pp {| indent_stack := [];
+              used_names := [];
+              output := "" |} with
+  | inl err => inl err
+  | inr (a, pps) => inr (a, output pps)
+  end.
+
+Definition get_indent : PrettyPrinter nat :=
+  fun pps => inr (hd 0 (indent_stack pps), pps).
+
+Definition update_indent (f : list nat -> list nat) : PrettyPrinter unit :=
+  fun pps => inr (tt, {| indent_stack := f (indent_stack pps);
+                         used_names := used_names pps;
+                         output := output pps |}).
+
+Definition push_indent (n : nat) : PrettyPrinter unit :=
+  update_indent (cons n).
+
+Definition pop_indent : PrettyPrinter unit :=
+  update_indent tl.
+
+Definition get_used_names : PrettyPrinter (list ident) :=
+  fun pps => inr (used_names pps, pps).
+
+Definition update_used_names (f : list ident -> list ident) : PrettyPrinter unit :=
+  fun pps => inr (tt, {| indent_stack := indent_stack pps;
+                         used_names := f (used_names pps);
+                         output := output pps |}).
+
+Definition push_use (n : ident) : PrettyPrinter unit :=
+  update_used_names (cons n).
+
+Definition pop_use : PrettyPrinter unit :=
+  update_used_names tl.
+
+Definition is_newline (c : ascii) : bool :=
+  match c with
+  | "010"%char => true
+  | _ => false
+  end.
+
+Definition last_line_length (s : string) : nat :=
+  (fix f (s : string) (result : nat) :=
+     match s with
+     | EmptyString => result
+     | String c s =>
+       if is_newline c then
+         f s 0
+       else
+         f s (S result)
+     end) s 0.
+
+Definition get_current_line_length : PrettyPrinter nat :=
+  fun pps => inr (last_line_length (output pps), pps).
+
+Definition update_output (f : string -> string) : PrettyPrinter unit :=
+  fun pps => inr (tt, {| indent_stack := indent_stack pps;
+                         used_names := used_names pps;
+                         output := f (output pps) |}).
+
+Definition append (s : string) : PrettyPrinter unit :=
+  update_output (fun o => o ++ s).
+
+Definition append_nl : PrettyPrinter unit := append nl.
+
+Definition append_indent : PrettyPrinter unit :=
+  indent <- get_indent;;
+  append (concat "" (repeat " " indent)).
+
+Definition append_nl_and_indent : PrettyPrinter unit :=
+  append_nl;; append_indent.
+
+Definition replace_char (orig : Ascii.ascii) (new : Ascii.ascii) : string -> string :=
+  fix f s :=
+    match s with
+    | EmptyString => EmptyString
+    | String c s => if (c =? orig)%char then
+                      String new (f s)
+                    else
+                      String c (f s)
+    end.
+
+Definition last_index_of (c : ascii) (s : string) : option nat :=
+  (fix f (s : string) (index : nat) (result : option nat) :=
+     match s with
+     | EmptyString => result
+     | String c' s =>
+       if (c' =? c)%char then
+         f s (S index) (Some index)
+       else
+         f s (S index) result
+     end) s 0 None.
+
+Definition to_upper (c : ascii) : ascii :=
+  match c with
+  | Ascii b0 b1 b2 b3 b4 b5 b6 b7 =>
+    Ascii b0 b1 b2 b3 b4 false b6 b7
+  end.
+
+Definition capitalize (s : string) : string :=
+  match s with
+  | EmptyString => EmptyString
+  | String c s => String (to_upper c) s
+  end.
+
+Definition printable_kername (name : kername) : string :=
+  match last_index_of "." name with
+  | Some n => substring (S n) (length name) name
+  | None => name
+  end.
+
+Definition kername_qualifier (name : kername) : string :=
+  match last_index_of "." name with
+  | Some n => substring 0 n name
+  | None => ""
+  end.
+
+Local Open Scope list.
+
+Local Definition indent_size := 2.
+
+Section FixExEnv.
+
+Context (Σ : Ex.global_env).
+
+Definition print_ty_name (name : kername) : PrettyPrinter unit :=
+  append (capitalize (printable_kername name)).
+
+Definition print_ctor_name (name : ident) : PrettyPrinter unit :=
+  append (capitalize name).
+
+Definition lookup_mind (name : kername) : option P.mutual_inductive_body :=
+  match Ex.lookup_env Σ name with
+  | Some (Ex.InductiveDecl mind) => Some mind
+  | _ => None
+  end.
+
+Definition lookup_ind_decl (ind : inductive) : PrettyPrinter P.one_inductive_body :=
+  match lookup_mind (inductive_mind ind) with
+  | Some {| P.ind_bodies := l |} =>
+    match nth_error l (inductive_ind ind) with
+    | Some body => ret body
+    | None => printer_fail ("could not find inductive " ++
+                            string_of_nat (inductive_ind ind) ++
+                            " in inductive " ++ inductive_mind ind)
+    end
+  | _ => printer_fail ("could not find " ++ inductive_mind ind ++ " in environment")
+  end.
+
+Definition print_ind_ctor (ind : inductive) (i : nat) : PrettyPrinter unit :=
+  oib <- lookup_ind_decl ind;;
+  match nth_error (P.ind_ctors oib) i with
+  | Some (name, _, _) =>
+    print_ctor_name name
+    (*append (replace_char "." "_" (inductive_mind ind) ++ "_" ++ name)*)
+  | None =>
+    printer_fail (inductive_mind ind ++ " does not have a ctor " ++ string_of_nat i)
+  end.
+
+Definition print_parenthesized
+           (parenthesize : bool)
+           (print : PrettyPrinter unit) : PrettyPrinter unit :=
+  if parenthesize then
+    append "(";; print;; append ")"
+  else
+    print.
+
+Definition parenthesize_app_head (t : term) : bool :=
+  match t with
+  | tLambda _ _
+  | tLetIn _ _ _
+  | tCase _ _ _
+  | tFix _ _ => true
+  | _ => false
+  end.
+
+Definition parenthesize_app_arg (t : term) : bool :=
+  match t with
+  | tLambda _ _
+  | tLetIn _ _ _
+  | tApp _ _
+  | tCase _ _ _
+  | tProj _ _
+  | tFix _ _ => true
+  | _ => false
+  end.
+
+Definition parenthesize_case_discriminee (t : term) : bool :=
+  match t with
+  | tLetIn _ _ _
+  | tCase _ _ _ => true
+  | _ => false
+  end.
+
+Definition parenthesize_case_branch (t : term) : bool :=
+  false.
+
+Definition fresh (name : ident) (used : list ident) : ident :=
+  if existsb (String.eqb name) used then
+    (fix f n i :=
+       match n with
+       | 0 => "unreachable"
+       | S n =>
+         let numbered_name := (name ++ string_of_nat i)%string in
+         if existsb (String.eqb numbered_name) used then
+           f n (S i)
+         else
+           numbered_name
+       end) (S (List.length used)) 2
+  else
+    name.
+
+Definition fresh_name (name : name) (Γ : list ident) : PrettyPrinter ident :=
+  used_names <- get_used_names;;
+  match name with
+  | nAnon => ret (fresh "_x" (Γ ++ used_names))
+  | nNamed name => ret (fresh name (Γ ++ used_names))
+  end.
+
+(*
+Definition blah :=
+  fix f x :=
+    match x with
+    | S x => (g x + f x)%nat
+    | 0 => 0
+    end
+ with g x :=
+      match x with
+      | S x => (g x + f x)%nat
+      | 0 => 0
+      end
+for f.
+
+Quote Recursively Definition foo := blah.
+*)
+
+Import P.
+Definition parenthesize_prod_domain (t : term) : bool :=
+  match t with
+  | tProd _ _ _ => true
+  | _ => false
+  end.
+
+Fixpoint print_type (t : term) : PrettyPrinter unit :=
+  match t with
+  | tInd ind _ => print_ty_name (inductive_mind ind)
+  | tProd _ dom cod =>
+    print_parenthesized (parenthesize_prod_domain dom) (print_type dom);;
+    append " -> ";;
+    print_type cod
+  | _ => printer_fail ("cannot print following as type" ++ nl ++ PCUICAstUtils.string_of_term t)
+  end.
+
+Import E.
+(* Print something of the form
+   foo =
+     a b c
+inlining lambdas (and fix points). For example, for
+   foo = \x \y \z -> z
+instead print
+   foo x y z = z
+*)
+Definition print_define_term
+         (Γ : list ident)
+         (name : ident)
+         (t : term)
+         (print_term : list ident -> term -> PrettyPrinter unit) : PrettyPrinter unit :=
+  name_col <- get_current_line_length;;
+  append name;;
+
+  let fix print_decompose Γ t :=
+      match t with
+      | tLambda arg_name t =>
+        arg_name <- fresh_name arg_name Γ;;
+        append (" " ++ arg_name);;
+        print_decompose (arg_name :: Γ) t
+      | _ =>
+        append " =";;
+        push_indent (name_col + indent_size);;
+        append_nl_and_indent;;
+        print_term Γ t;;
+        pop_indent
+      end in
+
+  match t with
+  | tFix [d] 0 => print_decompose (name :: Γ) (dbody d)
+  | _ => print_decompose Γ t
+  end.
+
+Fixpoint print_term (Γ : list ident) (t : term) : PrettyPrinter unit :=
+  match t with
+  | tBox _ => printer_fail "tBox"
+  | tRel n =>
+    match nth_error Γ n with
+    | Some name => append name
+    | None => printer_fail ("unbound tRel " ++ string_of_nat n)
+    end
+  | tVar ident => printer_fail ("tVar " ++ ident)
+  | tEvar _ _ => printer_fail "unexpected evar"
+  | tLambda name t =>
+    append "\";;
+
+    name <- fresh_name name Γ;;
+    append name;;
+    append " -> ";;
+    print_term (name :: Γ) t
+
+  | tLetIn name value body =>
+
+    let_col <- get_current_line_length;;
+    push_indent let_col;;
+
+    append "let";;
+
+    let print_and_add_one Γ name value :=
+        append_nl_and_indent;;
+        name <- fresh_name name Γ;;
+        (* We will define this name to make sure we don't reuse it
+           until the let is all over. Midlang does not allow shadowing. *)
+        push_use name;;
+        print_define_term Γ name value print_term;;
+        ret (name :: Γ) in
+
+    push_indent (let_col + indent_size);;
+
+    Γ <- print_and_add_one Γ name value;;
+
+    (* Print in Midlang/Elm style, which collapses multiple lets into one *)
+    (* Turned off because of Elm's insane shadowing rules *)
+    (*
+    num_collapsed <-
+    (fix print_lets Γ (t : term) :=
+       match t with
+       | tLetIn name value t =>
+         Γ <- print_and_add_one Γ name value;;
+         n <- print_lets Γ t;;
+         ret (S n)
+       | _ =>
+         pop_indent;; (* indent in let block *)
+
+         append_nl_and_indent;; (* indent to 'let' keyword *)
+         append "in";;
+
+         append_nl_and_indent;; (* body is indented to 'let'/'in' keyword as well *)
+         print_term Γ t;;
+         pop_indent;;
+         ret 0
+       end) Γ body;;
+
+    (* pop all the names we defined, we can reuse those names now. *)
+    monad_fold_left (fun _ _ => pop_use) (repeat tt (S num_collapsed)) tt
+    *)
+
+    pop_indent;;
+    append_nl_and_indent;;
+
+    append "in";;
+    append_nl_and_indent;;
+    print_term Γ body;;
+    pop_indent;;
+
+    pop_use
+
+  | tApp head arg =>
+    print_parenthesized (parenthesize_app_head head) (print_term Γ head);;
+    append " ";;
+    print_parenthesized (parenthesize_app_arg arg) (print_term Γ arg)
+
+  | tConst name => append (printable_kername name)
+  | tConstruct ind i => print_ind_ctor ind i
+
+  | tCase (ind, _) discriminee branches =>
+    case_col <- get_current_line_length;;
+    append "case ";;
+    print_parenthesized (parenthesize_case_discriminee discriminee)
+                        (print_term Γ discriminee);;
+    append " of";;
+
+    push_indent (case_col + indent_size);;
+
+    oib <- lookup_ind_decl ind;;
+
+    (* Take care that this is structurally recursive... *)
+    (fix print_branches (branches : list (nat * term)) (ctor_names : list ident) :=
+       match branches, ctor_names with
+       | [], [] => ret tt
+       | (arity, t) :: branches, ctor_name :: ctor_names =>
+         append_nl_and_indent;;
+
+         ctor_indent <- get_indent;;
+         push_indent (ctor_indent + indent_size);;
+
+         print_ctor_name ctor_name;;
+
+         (fix print_branch (n : nat) (Γ : list ident) (t : term) {struct t} :=
+            match n with
+            | 0 =>
+              append " ->";;
+              append_nl_and_indent;;
+              print_parenthesized (parenthesize_case_branch t) (print_term Γ t)
+
+            | S n =>
+              match t with
+              | tLambda name t =>
+                name <- fresh_name name Γ;;
+                append (" " ++ name);;
+                print_branch n (name :: Γ) t
+
+              | _ => printer_fail "could not decompose branch"
+              end
+            end) arity Γ t;;
+
+         pop_indent;;
+
+         print_branches branches ctor_names
+       | _, _ => printer_fail "wrong number of case branches compared to inductive"
+       end) branches (map (fun '(name, _, _) => name) (P.ind_ctors oib));;
+
+    pop_indent
+
+  | tProj _ _ => printer_fail "tProj"
+
+  | tFix mfix nfix =>
+    let_col <- get_current_line_length;;
+    push_indent let_col;;
+
+    (* Add names of fixes to context *)
+    Γ <- monad_fold_left
+           (fun Γ d => name <- fresh_name (dname d) Γ;;
+                       ret (name :: Γ)) mfix Γ;;
+    let names := rev (firstn (List.length mfix) Γ) in
+
+    append "let";;
+
+    push_indent (let_col + indent_size);;
+
+    (fix print_fixes (ds : list (def term)) (names : list ident) :=
+       match ds, names with
+       | [], _ => ret tt
+       | d :: ds, name :: names =>
+         append_nl_and_indent;;
+         print_define_term Γ name (dbody d) print_term;;
+         print_fixes ds names
+       | _, _ =>
+         printer_fail "unreachable"
+       end) mfix names;;
+
+    pop_indent;;
+
+    append_nl_and_indent;;
+    append "in";;
+    append_nl_and_indent;;
+    match nth_error names nfix with
+    | Some n => append n
+    | None => printer_fail "invalid fix index"
+    end;;
+
+    pop_indent
+
+  | tCoFix _ _ => printer_fail "Cannot handle cofix"
+  end.
+
+Definition print_constant_body (name : kername) (cst : Ex.constant_body) : PrettyPrinter unit :=
+  name_col <- get_current_line_length;;
+
+  push_indent name_col;;
+
+  let (type, body) := cst in
+
+  append (printable_kername name);;
+  append " : ";;
+  print_type type;;
+
+  match body with
+  | None => ret tt
+  | Some body =>
+    append_nl_and_indent;;
+    let name := printable_kername name in
+    push_use name;;
+    print_define_term [] name body print_term
+  end;;
+
+  pop_indent.
+
+Quote Recursively Definition foo := (5+5)%nat.
+
+Fixpoint decompose_ind_ctor (arity : nat) (ty : P.term) : PrettyPrinter (list P.term) :=
+  match arity with
+  | 0 => ret []
+  | S arity =>
+    match ty with
+    | P.tProd _ dom cod =>
+      tl <- decompose_ind_ctor arity cod;;
+      ret (dom :: tl)
+    | _ =>
+      printer_fail ("unexpected type of ctor: " ++ PCUICAstUtils.string_of_term ty)
+    end
+  end.
+
+Import P.
+Definition parenthesize_ind_ctor_ty (ty : term) : bool :=
+  match ty with
+  | tInd _ _
+  | tVar _ => false
+  | _ => true
+  end.
+
+Definition print_ind_ctor_definition
+           (ind_name : string)
+           (name : ident)
+           (ty : P.term)
+           (arity : nat) : PrettyPrinter unit :=
+  print_ctor_name name;;
+  tys <- decompose_ind_ctor arity ty;;
+
+  (fix f (tys : list P.term) (depth : nat) :=
+     match tys with
+     | [] => ret tt
+     | ty :: tys =>
+       append " ";;
+       match ty with
+       | tRel n =>
+         if (n =? depth)%nat then
+           print_ty_name ind_name
+          else
+            printer_fail ("cannot handle " ++ PCUICAstUtils.string_of_term ty ++ " in inductive")
+       | _ => print_parenthesized (parenthesize_ind_ctor_ty ty) (print_type ty)
+       end;;
+       f tys (S depth)
+     end) tys 0.
+
+Local Open Scope string.
+Definition print_mutual_inductive_body
+           (name : kername)
+           (mib : P.mutual_inductive_body) : PrettyPrinter unit :=
+  col <- get_current_line_length;;
+  push_indent col;;
+
+  let qualifier := kername_qualifier name in
+
+  (fix print_ind_bodies (l : list P.one_inductive_body) (first : bool) :=
+     match l with
+     | [] => ret tt
+     | oib :: l =>
+
+       (if first then ret tt else append_nl_and_indent);;
+
+       append "type ";;
+       let ind_name := qualifier ++ "." ++ P.ind_name oib in
+       print_ty_name ind_name;;
+
+       push_indent (col + indent_size);;
+
+       (fix print_ind_ctors (ctors : list (ident * P.term * nat)) prefix :=
+          match ctors with
+          | [] => ret tt
+          | (name, ty, arity) :: ctors =>
+            append_nl_and_indent;;
+            append (prefix ++ " ");;
+            print_ind_ctor_definition ind_name name ty arity;;
+
+            print_ind_ctors ctors "|"
+          end) (ind_ctors oib) "=";;
+
+       pop_indent;;
+
+       print_ind_bodies l false
+     end) (ind_bodies mib) true;;
+
+  pop_indent.
+
+Definition print_global_decl
+           (name : kername)
+           (decl : Ex.global_decl) : PrettyPrinter unit :=
+  match decl with
+  | Ex.ConstantDecl cst => print_constant_body name cst
+  | Ex.InductiveDecl mib => print_mutual_inductive_body name mib
+  end.
+
+Definition print_env : PrettyPrinter unit :=
+  sig_col <- get_current_line_length;;
+  push_indent sig_col;;
+
+  (fix f (l : Ex.global_env) (first : bool) :=
+     match l with
+     | (name, decl) :: l =>
+
+       (if first then ret tt else (append_nl;; append_nl_and_indent));;
+       print_global_decl name decl;;
+
+       f l false
+     | [] => ret tt
+     end) Σ true;;
+
+  pop_indent.
+End FixExEnv.
+
+Definition string_of_env_error Σ e :=
+  match e with
+  | IllFormedDecl s e =>
+    "IllFormedDecl " ++ s ++ "\nType error: " ++ string_of_type_error Σ e
+  | AlreadyDeclared s => "Alreadydeclared " ++ s
+  end%string.
+
+Definition wrap_EnvCheck {A} (ec : EnvCheck A) : PrettyPrinter A :=
+  match ec with
+  | CorrectDecl a => ret a
+  | EnvError Σ err =>
+    printer_fail ("EnvError: " ++ string_of_env_error Σ err)
+  end.
+
+Definition wrap_typing_result {A} (Σ : P.global_env) (tr : typing_result A) : PrettyPrinter A :=
+  match tr with
+  | Checked et => ret et
+  | TypeError te =>
+    printer_fail ("TypeError: " ++ string_of_type_error (P.empty_ext Σ) te)
+  end.
+
+Axiom assump : string -> forall {A}, A.
+
+Lemma wf_empty_ext (Σ : P.global_env) :
+  ∥PT.wf Σ∥ -> ∥PT.wf_ext (P.empty_ext Σ)∥.
+Proof.
+  intros [wfΣ].
+  constructor.
+  split; [assumption|].
+  todo "on_udecl on empty_ext".
+Qed.
+
+Lemma proj_wf
+      {Σ : P.global_env_ext}
+      (wfΣ : ∥PT.wf_ext Σ∥) : ∥PT.wf Σ.1∥.
+Proof. firstorder. Qed.
+
+Definition erase_and_debox_single
+           (Σ : P.global_env_ext)
+           (wfΣ : ∥PT.wf_ext Σ∥)
+           (decl : P.global_decl) : PrettyPrinter Ex.global_decl :=
+  match decl with
+  | P.ConstantDecl cst =>
+    let (type, body, _) := cst in
+    ebody <- match body with
+             | None => ret None
+             | Some body =>
+               ebody <- wrap_typing_result
+                          Σ.1
+                          (EF.erase Σ wfΣ [] body (assump "assuming well-typedness"));;
+               result <- wrap_EnvCheck (check_applied Σ.1 ebody (proj_wf wfΣ));;
+               if result then
+                 ret (Some (debox_all ebody))
+               else
+                 printer_fail "Not all constructors or constants are appropriately applied"
+             end;;
+    ret (Ex.ConstantDecl {| Ex.cst_type := type; Ex.cst_body := ebody |})
+  | P.InductiveDecl mib =>
+    (*mib <- wrap_typing_result
+             Σ.1
+             (EF.erase_mutual_inductive_body Σ wfΣ mib);;*)
+    ret (Ex.InductiveDecl mib)
+  end.
+
+(* Extract the specified environment to Midlang, creating definitions for all symbols. *)
+Definition extract_env (Σ : T.global_env) : PrettyPrinter unit :=
+  let Σ := fix_global_env_universes Σ in
+  let Σ := (T2P.trans_global (T.empty_ext Σ)).1 in
+  G <- wrap_EnvCheck (check_wf_env_only_univs Σ);;
+  let wfΣ := G.π2.p2 in
+  let Σext := P.empty_ext Σ in
+  let wfΣext : ∥PT.wf_ext Σext∥ := wf_empty_ext Σ wfΣ in
+  Σex <- monad_map (fun '(name, decl) =>
+                      decl <- erase_and_debox_single Σext wfΣext decl;;
+                      ret (name, decl)) Σ;;
+  print_env Σex.
+
+Local Open Scope nat.
+
+Inductive Msg :=
+| increment
+| decrement.
+
+(*
+Quote Recursively Definition test :=
+  (fun (state : nat) (maybe_msg : option Msg) =>
+    match maybe_msg with
+    | Some increment => Some (state + 1)
+    | Some decrement => Some (state - 1)
+    | _ => None
+    end).
+*)
+
+Definition app (f : nat -> nat) (n : nat) : nat :=
+  f n.
+
+Definition test : nat :=
+  let x := 5 in
+  let foo n := S n in
+  let even :=
+      fix even n :=
+        match n with
+        | 0 => true
+        | S n => odd n
+        end
+     with odd n :=
+        match n with
+        | 0 => false
+        | S n => even n
+        end
+      for even in
+  let fix even n :=
+      match n with
+      | 0 => true
+      | 1 => false
+      | S (S n) => even n
+      end in
+  let y := 7 in
+  x + app (fun x => S x) (foo 3) + y + foo (foo x) + if even x then 2 else 0.
+
+Definition test' : bool :=
+  let x := let y := true in y in
+  let y := x in y.
+
+Quote Recursively Definition test_program := test.
+
+Local Open Scope string.
+Definition test3 :=
+  match finish_print (append_nl;; extract_env test_program.1) with
+  | inl err => "Printer error: " ++ err
+  | inr (_, output) => output
+  end.
+
+Compute test3.
+
+Compute erase_check_debox_all_print [] "foo" [] test_program.
+
+Definition test2 : string :=
+  match erase_check_debox_all [] test_program with
+  | CorrectDecl (Σ, (args, term)) =>
+    match finish_print (append_nl;; print_term Σ ["f"] term) with
+    | inl err => "Printer error: " ++ err
+    | inr (_, output) => output
+    end
+  | EnvError Σ (AlreadyDeclared id) => "Already declared: " ++ id
+  | EnvError Σ (IllFormedDecl id e) =>
+    "Type error: " ++ PCUICSafeChecker.string_of_type_error Σ e ++ ", while checking " ++ id
+  end.
+
+Compute test2.
